theories/case_studies/droe/deep_immutability_adequacy.v
@@ -6,14 +6,13 @@ From cap_machine Require Import mkregion_helpers.
 From cap_machine Require Import region_invariants_revocation region_invariants_allocation.
 From iris.program_logic Require Import adequacy.
 From iris.base_logic Require Import invariants.
-From cap_machine Require Import compartment_layout switcher_adequacy.
 From cap_machine Require Import disjoint_regions_tactics.
 From cap_machine Require Import switcher_preamble interp_switcher_call interp_switcher_return.
+From cap_machine Require Import compartment_layout switcher_adequacy.
 
 Class memory_layout `{MP: MachineParameters} := {
 
     (* switcher *)
-    switcher_layout : @switcherLayout MP;
     switcher_cmpt : cmptSwitcher;
 
     (* assert *)
@@ -41,6 +40,25 @@ Class memory_layout `{MP: MachineParameters} := {
     assert_switcher_disjoint assert_cmpt switcher_cmpt;
   }.
 
+Local Instance memory_layout_switcherLayout `{memory_layout} : switcherLayout.
+Proof.
+  exact (cmptSwitcher_switcherLayout switcher_cmpt).
+Defined.
+
+Local Instance memory_layout_switcherLayoutWf `{memory_layout} : switcherLayoutWf.
+Proof.
+  pose proof (ot_switcher_size switcher_cmpt).
+  pose proof (switcher_size switcher_cmpt).
+  pose proof (switcher_call_entry_point switcher_cmpt).
+  pose proof (switcher_return_entry_point switcher_cmpt).
+  refine (mkSwitcherLayoutWf _ _ _ _ _); cbn in *; auto.
+Defined.
+
+Local Instance memory_layout_assertLayout `{memory_layout} : assertLayout.
+Proof.
+  exact (cmptAssert_assertLayout assert_cmpt).
+Defined.
+
 Definition mk_initial_memory `{memory_layout} (mem: Mem) :=
   mk_initial_switcher switcher_cmpt ∪
     mk_initial_assert assert_cmpt ∪
@@ -56,15 +74,15 @@ Definition is_initial_registers `{memory_layout} (reg: Reg) :=
 
 Program Definition is_initial_sregisters `{@memory_layout MP} (sreg : SReg) :=
   sreg !! MTDC = Some (WCap RWL Local
-                         (@b_trusted_stack MP switcher_layout)
-                         (@e_trusted_stack MP switcher_layout)
-                         (@b_trusted_stack MP switcher_layout)).
+                         (b_trusted_stack switcher_cmpt)
+                         (e_trusted_stack switcher_cmpt)
+                         (b_trusted_stack switcher_cmpt)).
 
 Definition is_initial_memory `{@memory_layout MP} (mem: Mem) :=
-  let b_switcher := (@b_switcher MP switcher_layout) in
-  let e_switcher := (@e_switcher MP switcher_layout) in
-  let a_switcher_call := (@a_switcher_call MP switcher_layout) in
-  let ot_switcher := (@ot_switcher MP switcher_layout) in
+  let b_switcher := (b_switcher switcher_cmpt) in
+  let e_switcher := (e_switcher switcher_cmpt) in
+  let a_switcher_call := (a_switcher_call switcher_cmpt) in
+  let ot_switcher := (ot_switcher switcher_cmpt) in
   let switcher_entry :=
     WSentry XSRW_ Local
       b_switcher
@@ -80,12 +98,7 @@ Definition is_initial_memory `{@memory_layout MP} (mem: Mem) :=
 
   mem = mk_initial_memory mem
   (* instantiating main *)
-  ∧ (cmpt_imports main_cmpt) =
-    droe_main_imports
-      b_switcher e_switcher
-      a_switcher_call ot_switcher
-      (b_assert assert_cmpt) (e_assert assert_cmpt)
-      C_f
+  ∧ (cmpt_imports main_cmpt) = droe_main_imports C_f
   ∧ (cmpt_code main_cmpt) = droe_main_code
   ∧ (cmpt_data main_cmpt) = droe_main_data
   ∧ (cmpt_exp_tbl_entries main_cmpt) = []
@@ -164,17 +177,6 @@ Section Adequacy.
                   (state_is_good (reg', sreg', m'))).
     eapply WPI. 2: assumption. intros Hinv κs. clear WPI.
 
-    set b_switcher := (@b_switcher MP switcher_layout).
-    set e_switcher := (@e_switcher MP switcher_layout).
-    set a_switcher_call := (@a_switcher_call MP switcher_layout).
-    set ot_switcher := (@ot_switcher MP switcher_layout).
-    set a_switcher_return := (@a_switcher_return MP switcher_layout).
-    set b_trusted_stack := (@b_trusted_stack MP switcher_layout).
-    set e_trusted_stack := (@e_trusted_stack MP switcher_layout).
-    set switcher_size := (@switcher_size MP switcher_layout).
-    set switcher_call_entry_point := (@switcher_call_entry_point MP switcher_layout).
-    set switcher_return_entry_point := (@switcher_return_entry_point MP switcher_layout).
-
     pose proof Hm as Hm'.
     destruct Hm as (Hm
                     & main_imports & main_code & main_data & main_exp_tbl
@@ -184,7 +186,7 @@ Section Adequacy.
     iMod (gen_heap_init (reg:Reg)) as (reg_heapg) "(Hreg_ctx & Hreg & _)".
     iMod (gen_heap_init (sreg:SReg)) as (sreg_heapg) "(Hsreg_ctx & Hsreg & _)".
     iMod (gen_heap_init (m:Mem)) as (mem_heapg) "(Hmem_ctx & Hmem & _)".
-    iMod (seal_store_init ({[ ot_switcher ]} : gset _)) as (seal_storeg) "Hseal_store".
+    iMod (seal_store_init ({[ (ot_switcher switcher_cmpt) ]} : gset _)) as (seal_storeg) "Hseal_store".
     set (
         C_f :=
        (WCap RO Global (cmpt_exp_tbl_pcc C_cmpt) (cmpt_exp_tbl_entries_end C_cmpt)
@@ -194,8 +196,8 @@ Section Adequacy.
     iMod (
        entry_init (
            {[
-               (seal_capability C_f ot_switcher) := 1;
-               (borrow (seal_capability C_f ot_switcher)) := 1
+               (seal_capability C_f (ot_switcher switcher_cmpt)) := 1;
+               (borrow (seal_capability C_f (ot_switcher switcher_cmpt))) := 1
            ]}
 
          )
@@ -228,10 +230,9 @@ Section Adequacy.
 
     pose ceriseg := CeriseG Σ Hinv mem_heapg reg_heapg sreg_heapg entry_g.
     pose logrel_na_invs := Build_logrel_na_invs _ na_invg logrel_nais.
-    pose switcher_layout_g := (@switcher_layout MP Layout).
 
     pose proof (
-        @droe_spec Σ ceriseg seal_storeg _ _ _ logrel_na_invs _ _  switcher_layout_g C
+        @droe_spec Σ ceriseg seal_storeg _ _ _ logrel_na_invs _ _ _ _ _ C
       ) as Spec.
 
     (* Get initial sregister mtdc *)
@@ -298,9 +299,7 @@ Section Adequacy.
 
     rewrite /cmpt_switcher_code_mregion.
     iDestruct (big_sepM_union with "Hswitcher") as "[Hswitcher_sealing Hswitcher]".
-    { eapply cmpt_switcher_code_stack_mregion_disjoint ; eauto.
-      exact switcher_cmpt.
-    }
+    { eapply cmpt_switcher_code_stack_mregion_disjoint ; eauto. }
     iEval (rewrite /mkregion) in "Hswitcher_sealing".
     rewrite finz_seq_between_singleton.
     2: { apply switcher_call_entry_point. }
@@ -316,11 +315,10 @@ Section Adequacy.
     iAssert ( switcher_preamble.switcher_inv )
       with "[Hswitcher Hswitcher_sealing Htrusted_stack Hcstk_full Hmtdc]" as "Hswitcher".
     {
-      rewrite /switcher_preamble.switcher_inv /codefrag /region_pointsto.
-      replace (a_switcher_call ^+ length switcher_instrs)%a
-        with e_switcher.
-      2: { pose proof switcher_size as H.
-           subst a_switcher_call e_switcher.
+      rewrite /switcher_preamble.switcher_inv /codefrag /region_pointsto /=.
+      replace ((a_switcher_call switcher_cmpt) ^+ length switcher_instrs)%a
+        with (e_switcher switcher_cmpt).
+      2: { pose proof (switcher_size switcher_cmpt) as H.
            solve_addr+H.
       }
       iFrame "∗#".
@@ -333,7 +331,6 @@ Section Adequacy.
       iDestruct "Htrusted_stack" as "[Hbase_stack Htrusted_stack]".
       iFrame.
       iSplitL; last (iPureIntro ; by rewrite finz_add_0).
-      subst switcher_layout_g.
       iSplit; iPureIntro; solve_addr.
     }
     iMod (na_inv_alloc logrel.logrel_nais _ switcherN _ with "Hswitcher") as "#Hswitcher".
@@ -495,7 +492,7 @@ Section Adequacy.
       iApply (monoReq_interp _ _ _ _ Temporary); done.
     }
 
-    iAssert ( interp Winit_C C (WSealed ot_switcher C_f)) with
+    iAssert ( interp Winit_C C (WSealed (ot_switcher switcher_cmpt) C_f)) with
       "[HC_code Hr_C HC_data Hsts_C Hentry_Cf']" as "#Hinterp_C".
     { iApply (ot_switcher_interp_entry _ _ _ _ 1 1); eauto; last lia.
       pose proof (cmpt_exp_tbl_entries_size C_cmpt) as H1.
@@ -544,7 +541,7 @@ Section Adequacy.
     iDestruct (big_sepM_delete _ _ cgp with "Hreg") as "[Hcgp Hreg]"; first by simplify_map_eq.
     iDestruct (big_sepM_delete _ _ csp with "Hreg") as "[Hcsp Hreg]"; first by simplify_map_eq.
 
-    iPoseProof (Spec _ _ _ _ _ _ _ _
+    iPoseProof (Spec _ _ _ _ _
                   _ _ _ _ _
                   [] [] assertN switcherN []
                  with "[ $Hassert $Hswitcher $Hna
