theories/case_studies/stack_object/stack_object_spec_closure.v
@@ -17,7 +17,7 @@ Section SO.
     {nainv: logrel_na_invs Σ}
     {cstackg : CSTACKG Σ}
     `{MP: MachineParameters}
-    {swlayout : switcherLayout}
+    {swlayout : switcherLayout} {swlayoutWf : switcherLayoutWf} {assertlayout : assertLayout}
   .
 
   Context {C : CmptName}.
@@ -76,7 +76,6 @@ Section SO.
     (b_so_exp_tbl e_so_exp_tbl : Addr)
     (g_so_exp_tbl : Locality)
 
-    (b_assert e_assert : Addr) (a_flag : Addr)
     (C_f : Sealable)
 
     (W : WORLD)
@@ -85,10 +84,7 @@ Section SO.
 
     :
 
-    let imports :=
-     so_main_imports
-       b_switcher e_switcher a_switcher_call ot_switcher b_assert e_assert C_f
-    in
+    let imports := so_main_imports C_f in
 
     Nswitcher ## Nassert ->
     Nswitcher ## Nso ->
@@ -1526,7 +1522,6 @@ Section SO.
 
     (b_so_exp_tbl e_so_exp_tbl : Addr)
 
-    (b_assert e_assert : Addr) (a_flag : Addr)
     (C_f : Sealable)
 
     (W : WORLD)
@@ -1535,10 +1530,7 @@ Section SO.
 
     :
 
-    let imports :=
-     so_main_imports
-       b_switcher e_switcher a_switcher_call ot_switcher b_assert e_assert C_f
-    in
+    let imports := so_main_imports C_f in
 
     Nswitcher ## Nassert ->
     Nswitcher ## Nso ->
