theories/case_studies/vae/vae_spec.v
@@ -14,7 +14,7 @@ Section VAE.
     {nainv: logrel_na_invs Σ}
     {cstackg : CSTACKG Σ}
     `{MP: MachineParameters}
-    {swlayout : switcherLayout}
+    {swlayout : switcherLayout} {swlayoutWf : switcherLayoutWf} {assertlayout : assertLayout}
   .
 
   Context {C : CmptName}.
@@ -32,7 +32,6 @@ Section VAE.
 
     (b_vae_exp_tbl e_vae_exp_tbl : Addr)
 
-    (b_assert e_assert : Addr) (a_flag : Addr)
     (C_f : Sealable)
 
     (W0 : WORLD)
@@ -46,10 +45,7 @@ Section VAE.
     (i : positive)
     :
 
-    let imports :=
-     vae_main_imports
-       b_switcher e_switcher a_switcher_call ot_switcher b_assert e_assert C_f
-    in
+    let imports := vae_main_imports C_f in
 
     Nswitcher ## Nassert ->
     Nswitcher ## Nvae_code ->
@@ -59,7 +55,7 @@ Section VAE.
 
     dom rmap = all_registers_s ∖ {[ PC ; cgp ; csp]} ->
     (forall r, r ∈ (dom rmap) -> is_Some (rmap !! r) ) ->
-    SubBounds pc_b pc_e pc_a (pc_a ^+ length (vae_main_code ot_switcher))%a ->
+    SubBounds pc_b pc_e pc_a (pc_a ^+ length vae_main_code)%a ->
 
     (cgp_b + length vae_main_data)%a = Some cgp_e ->
     (pc_b + length imports)%a = Some pc_a ->
@@ -70,7 +66,7 @@ Section VAE.
       na_inv logrel_nais Nassert (assert_inv b_assert e_assert a_flag)
       ∗ na_inv logrel_nais Nswitcher switcher_inv
       ∗ na_inv logrel_nais Nvae_code
-          ([[ pc_b , pc_a ]] ↦ₐ [[ imports ]] ∗ codefrag pc_a (vae_main_code ot_switcher))
+          ([[ pc_b , pc_a ]] ↦ₐ [[ imports ]] ∗ codefrag pc_a vae_main_code)
       ∗ inv (export_table_PCCN VAEN) (b_vae_exp_tbl ↦ₐ WCap RX Global pc_b pc_e pc_b)
       ∗ inv (export_table_CGPN VAEN) ((b_vae_exp_tbl ^+ 1)%a ↦ₐ WCap RW Global cgp_b cgp_e cgp_b)
       ∗ inv (export_table_entryN VAEN (b_vae_exp_tbl ^+ 2)%a)
