theories/switcher/interp_switcher_call.v
@@ -19,7 +19,7 @@ Section fundamental.
     {stsg : STSG Addr region_type Σ} {cstackg : CSTACKG Σ} {heapg : heapGS Σ}
     {nainv: logrel_na_invs Σ}
     `{MP: MachineParameters}
-    {swlayout : switcherLayout}
+    {swlayout : switcherLayout} {swlayoutwf : switcherLayoutWf}
   .
 
   Implicit Types W : WORLD.
